---
date: 2025-07-13
relevant-topics: 
- sequences
- recursion
- simultaneous equations
---

A sequence is defined by $u_{n + 2} = 3u_{n + 1} - 2u_{n}$ with $u_{1} = 2$ and $u_{2} = 5$.

a)  Find $u_{3}$ and $u_{4}$.

b)  Write down a definition for the sequence in the form

$$
u_{n+1} = au_{n} + b.
$$

## Solution

$u_{3}$ and $u_{4}$ can be found by substituting the correct terms into the given definition of the sequence.

\begin{align}
    u_{3}   &= 3u_{2} - 2u_{1} \\
            &= 3(5) - 2(2) \\
            &= 11 \\
    u_{4}   &= 3u_{3} - 2u_{2} \\
            &= 3(11) - 2(5) \\
            &= 23
\end{align}

For part (b), the two unknowns $a$ and $b$ can be found using simultaneous equations. We can derive these equations by substituting two pairs of terms into the new definition. For example, substituting $u_{1} = 2$ and $u_{2} = 5$ yields 

$$
2a + b = 5,
$$

and $u_{2} = 5$ and $u_{3} = 11$ yields 
$$
5a + b = 11.
$$

Solving this system of equations yields $a = 2$ and $b = 1$. You can check that this answer is indeed correct by substituting the values of $u_{3}$ and $u_{4}$ into the new definition.